Typing preservation proof. case fieldAccess.

CIFC.backup.v
@@ -7,7 +7,6 @@ Require Import Coq.Lists.List.
 
 Require Import Label.
 
-
 (* identifiers *)
 Inductive id : Type :=
   | Id : string -> id.
@@ -18,10 +17,6 @@ Inductive cn : Type :=
 
 Inductive field : Type :=
   | fd : cn -> id -> field.
-
-
-
-
 
 (* comparison of identifiers *)
 Definition beq_id x y :=
@@ -80,10 +75,10 @@ Inductive value : tm -> Prop :=
   | v_label :
       forall lb, value (l lb)
   | v_labeled : forall v lb,
-      value v ->
+     (* value v ->*)
       value (v_l v lb)
   | v_opa_labeled : forall v lb,
-      value v ->
+     (* value v ->*)
       value (v_opa_l v lb).
 
 Inductive Exception : tm -> Prop :=
@@ -356,7 +351,6 @@ Inductive step : tm -> Sigma -> tm -> Sigma -> Prop :=
       (unlabel e) / sigma ==> (unlabel e') / sigma'
   (* unlabel *)
   | ST_unlabel2 : forall sigma v lb l' sigma' s h s',
-      value v ->
       sigma = SIGMA s h ->
       l' = join_label lb (current_label sigma) ->
       s' = update_current_label s l'-> 
@@ -501,13 +495,14 @@ Inductive step : tm -> Sigma -> tm -> Sigma -> Prop :=
        Some v1 = sf(id1) ->
        Some v2 = sf(id2) ->
        v1 <> v2 ->
-       If id1 id2 s1 s2 / sigma ==>  s1 / sigma
+       If id1 id2 s1 s2 / sigma ==>  s2 / sigma
 (* sequence *)
    (* context rule *)
   | ST_seq1 : forall sigma s1 s2 s1', 
     Sequence s1 s2 / sigma ==> Sequence s1' s2 / sigma
    (* sequence rule *)
   | ST_seq2 : forall sigma v s , 
+    value v->
     Sequence v s / sigma ==> s / sigma
 
 where "c1 '/' st '==>' c1' '/' st'" := (step c1 st c1' st').
@@ -661,15 +656,14 @@ Inductive wfe_heap : Class_table -> typing_context -> heap -> Prop :=
 
 Inductive wfe_heap : Class_table -> typing_context -> heap -> Prop :=
   | empty_heap_wfe : forall ct ctx, wfe_heap ct ctx empty_heap
-  | heap_wfe : forall h h' o cls_def F cn ct gamma fields ho lo,
+  | heap_wfe : forall h h' o cls_def F ct gamma cn ho lo method_defs field_defs,
         h(o) = None ->
         wfe_heap ct gamma h ->
         ho = Some (Heap_OBJ cls_def F lo) ->
         h' = (fun x' => if beq_oid o x' then ho else (h x')) ->
-        (* cls = class_def cn field_defs method_defs-> *)
         Some cls_def  = ct cn ->
-        fields = (find_fields cls_def) ->
-        (forall f cls', type_of_field fields f = Some cls' -> exists v, F(f) = Some v)->
+        cls_def = class_def cn field_defs method_defs ->
+        (forall f cls', type_of_field field_defs f = Some cls' -> exists v, F(f) = Some v)->
         (exists o', h' o' = None) ->
         wfe_heap ct gamma h'.
 
@@ -698,15 +692,18 @@ Proof with auto.
 Qed.
 
 (*
-Inductive wfe_heap : Class_table -> typing_context -> heap -> Prop :=
-  | empty_heap_wfe : forall ct ctx, wfe_heap ct ctx empty_heap
-  | heap_wfe : forall h o cls F cn field_defs method_defs ct ctx h' lo,
-      h(o) = Heap_OBJ cls F lo ->
-      cls = class_def cn field_defs method_defs->
-      Some cls  = ct cn ->
-      F (x) ->
-      h' = (add_heap_obj h o (Heap_OBJ cls F lo)) ->
-      wfe_heap ct ctx h'.
+Lemma field_val_of_heap_obj : forall cls_name h o gamma CT cls_def F lo cls' field_defs method_defs,
+  wfe_heap CT gamma h -> 
+  h(o) = Some (Heap_OBJ cls_def F lo) ->
+  cls_def =  (class_def cls_name field_defs method_defs) ->
+  CT cls_name = Some cls_def ->
+  (forall f, type_of_field field_defs f = Some cls' -> exists v, F(f) = Some v).
+Proof with auto.
+  intros. induction H. inversion H0. case_eq (beq_oid o0 o). intro.
+  rewrite -> H6 in H0. rewrite -> H11 in H0. subst. inversion H0. subst.
+  apply H9 with (f:=f) (cls':=cls'). assumption.
+  intros. rewrite -> H6 in H0. rewrite -> H11 in H0. apply IHwfe_heap. assumption. assumption.
+Qed.
 *)
 
 
@@ -718,21 +715,18 @@ Proof with auto.
   auto. destruct H. destruct H. destruct H. inversion H.
 Qed.
 
-Lemma heap_consist_ct : forall h o ct ctx cls F lo, 
+Lemma heap_consist_ct : forall h o ct ctx cls F lo ,
   wfe_heap ct ctx h -> 
   h(o) = Some (Heap_OBJ cls F lo) ->
-  exists cn cls_def, ct cn = Some (cls_def).
+  exists cn field_defs method_defs, ct cn = Some cls /\ cls = (class_def cn field_defs method_defs).
 Proof with auto.
-  intros. inversion H.  
-  - subst. inversion H0. 
-  - subst. exists cn0. exists cls_def. auto.
+  intros. induction H. 
+  - inversion H0.
+  - case_eq (beq_oid o0 o).  intros. rewrite -> H3 in H0. rewrite -> H8 in H0.  
+      exists cn0. exists  field_defs. exists method_defs. rewrite -> H0 in H2. inversion H2.
+      split.  auto.  auto. 
+    intro. rewrite ->H3 in H0. rewrite -> H8 in H0. apply IHwfe_heap. auto. 
 Qed.
-
-Lemma ct_consist_heap : forall h o ct ctx cls F lo, 
-  wfe_heap ct ctx h -> 
-  
-  h(o) = Some (Heap_OBJ cls F lo) ->
-  exists cn field_defs method_defs, ct cn = Some (class_def cn field_defs method_defs).
 
 Fixpoint variable_exists (s : stack) (x : id) :=
   match s with 
@@ -744,10 +738,10 @@ Fixpoint variable_exists (s : stack) (x : id) :=
   end.
 
 Inductive wfe_stack_frame : heap -> labeled_stack_frame -> Prop :=
-  | stack_frame_wfe : forall h lsf sf v o lb cls_def F lo,
+  | stack_frame_wfe : forall h lsf sf o lb,
         lsf = Labeled_frame lb sf ->
-        (forall x, sf x = Some v ->
-        v = null \/ ((v = ObjId o) -> h(o) = Some (Heap_OBJ cls_def F lo)) \/ v = l lb) ->
+        (forall x v, sf x = Some v ->
+        v = null \/ ( v = ObjId o /\ (exists F lo cls_def, h(o) = Some (Heap_OBJ cls_def F lo)) )) ->
         wfe_stack_frame h lsf. 
 
 
@@ -779,7 +773,7 @@ Proof.
   - intro. intro. rewrite -> H0 in H. inversion H. 
 Qed.
 
-Lemma Typed_variable : forall sigma s h ct gamma x T lb sf s',
+Lemma Typed_variable : forall sigma s h ct gamma x T sf s' lb,
   sigma = SIGMA s h ->
   wfe_stack ct gamma h s ->
    gamma x = Some T -> 
@@ -814,15 +808,6 @@ Proof with eauto.
 Qed. 
 
 Check f_equal.
-
-Lemma beq_equal : forall x x', beq_id x x' = true -> x' = x.
-Proof.
-   intros. unfold beq_id in H. 
-  destruct x. destruct x'.  f_equal.
- case_eq (string_dec s s0). 
-  - intros. rewrite -> e. auto.
-  - intro. intro. rewrite -> H0 in H. inversion H. 
-Qed.
 
 Lemma wfe_oid : forall o ct gamma s h sigma cls_def cn, 
   sigma = SIGMA s h ->
@@ -932,10 +917,14 @@ Proof with auto.
        apply wfe_oid with (o:=o) (ct:=CT) (gamma:=Gamma) (s:=s) (h:=h) 
                           (sigma:=sigma) (cls_def:=cls_def) (cn:=clsT). auto. auto. auto. auto. 
        destruct H8 as [F]. destruct H8 as [lb].
+
       assert (exists v, F(f) = Some v).
       apply field_val_of_heap_obj with (h:=h) (o:=o) (gamma:=Gamma) (CT:=CT) 
                               (cls_def:=cls_def) (F:=F) (lo:=lb) (cls':=cls') (fields:=fields_def).
       auto. auto. auto. auto. auto. 
+
+
+
       destruct H9 as [v].
       remember (join_label lb (current_label sigma)) as l'.
       remember (update_current_label s l') as s'.
@@ -952,10 +941,10 @@ Proof with auto.
     rewrite <- H7 in H2. inversion H2.
    
      (* call field access on labeled value*)
-    {rewrite <- H8  in H2. inversion H2. }
+    {rewrite <- H7  in H2. inversion H2. }
     
      (* call field access on opaque label value*)
-    {rewrite <- H8  in H2. inversion H2. }
+    {rewrite <- H7  in H2. inversion H2. }
 
      (* context rule *)
     + { destruct H6 as [e']. destruct H6 as [sigma'].
@@ -1030,7 +1019,7 @@ Proof with auto.
               apply ST_MethodCallException with (sigma:=(SIGMA s h)) (v:=argu) (meth:=meth).
 
                   subst. inversion H2_.
-                rewrite <- H7 in H2_. inversion H2_.                 rewrite <- H7 in H2_. inversion H2_. 
+                rewrite <- H6 in H2_. inversion H2_.                 rewrite <- H6 in H2_. inversion H2_. 
       +  destruct H5 as [t']. destruct H5 as [sigma']. exists (MethodCall t' meth argu). exists (sigma').   
                   apply ST_MethodCall1 with (sigma:=sigma) (sigma':=sigma') (e2:=argu) (e:=e) (e':=t') (id:=meth). apply H5.
 
@@ -1118,7 +1107,7 @@ Proof with auto.
                 auto. auto. auto. auto. auto.
 
             (* subgoal #3 *)
-                rewrite <- H5 in H2.  inversion H2. 
+                rewrite <- H4 in H2.  inversion H2. 
 
              (* subgoal #4 *)
                 + destruct H3 as [t']. destruct H3 as [sigma']. 
@@ -1136,7 +1125,7 @@ Proof with auto.
                     
                    exists (l lb). exists (sigma). apply ST_labelof2 with (v:=v) (lb:=lb).
 
-                    rewrite <- H5 in H2. inversion H2. 
+                    rewrite <- H4 in H2. inversion H2. 
              (* subgoal #2 *)
                 + destruct H3 as [t']. destruct H3 as [sigma']. 
                     exists  (labelOf t'). exists sigma'. apply ST_labelof1 with (sigma:=sigma) (sigma':=sigma') (e:=e) (e':=t'). auto. 
@@ -1150,7 +1139,7 @@ Proof with auto.
                     exists NPE. exists sigma.  apply ST_unlabel_opaqueDataException with (sigma:=sigma).
                     rewrite <- H4 in H2.  inversion H2.
               
-                     rewrite <- H5 in H2. inversion H2. 
+                     rewrite <- H4 in H2. inversion H2. 
  
                 remember ( join_label lb (current_label sigma)) as l'.
                 remember (update_current_label s l') as s'.
@@ -1389,8 +1378,8 @@ Proof with auto.
                   auto. auto. 
 
                   rewrite <- H5 in H2_. inversion H2_.
-                  rewrite <- H6 in H2_. inversion H2_.
-                  rewrite <- H6 in H2_. inversion H2_.
+                  rewrite <- H5 in H2_. inversion H2_.
+                  rewrite <- H5 in H2_. inversion H2_.
      
       + destruct  IHhas_type2.  auto. auto. auto. auto. 
           destruct H4 as [t']. destruct H4 as [sigma']. 
@@ -1404,30 +1393,162 @@ Proof with auto.
           auto. 
 
 (* if *)
-- destruct  IHhas_type1; auto.  destruct  IHhas_type2; auto. 
-   inversion H2.  inversion H1. subst. inversion H3. 
-   subst. 
-    destruct  IHhas_type3; auto. destruct  IHhas_type4; auto.
+- (*destruct  IHhas_type1; auto.  destruct  IHhas_type2; auto. *)
+  inversion H2. inversion H1. subst. inversion H3. 
+  assert (exists v1, sf id1 = Some v1). 
+  apply Typed_variable with (sigma:=(SIGMA (s) h)) (s:=s) (h:=h) (ct:=CT) 
+                                            (gamma:=Gamma) (x:=id1) (T:=(classTy T)) (lb:=lb) (sf:=sf) (s':=s').
+  auto. auto. auto. auto. 
+  assert (exists v2, sf id2 = Some v2). 
+  apply Typed_variable with (sigma:=(SIGMA (s) h)) (s:=s) (h:=h) (ct:=CT) 
+                                            (gamma:=Gamma) (x:=id2) (T:=(classTy T)) (lb:=lb) (sf:=sf) (s':=s').
+  auto. auto. auto. auto. 
 
-    case (e1 = e2).
+  destruct H19 as [v1].   destruct H20 as [v2].
+  right. inversion H8. inversion H21. destruct H22 with id1 v1. 
+  rewrite <- H27; auto. destruct H22 with id2 v2.  destruct H22 with id1 v1.  
+  rewrite <- H27; auto. rewrite <- H27; auto. rewrite <- H27; auto. 
+  
+  exists s1. exists sigma.
+  apply ST_if_b1 with (sigma:=sigma) (s1:=s1) (s2:=s2) (v1:=v1) (v2:=v2)
+                                (s:=s) (h:=h) (lsf:=lsf) (s':=s') (lb:=lb) (sf:=sf) (id1:=id1) (id2:=id2). 
+  auto. rewrite <- H24 in H4. assumption. auto. auto. auto. subst. auto. 
+  destruct H28.
 
-           + subst. exists v. exists (SIGMA (Labeled_frame lb sf :: s') h).
-
-      apply ST_var with 
-      (id:=x) (lb:=lb) (sf:=sf) (lsf:=Labeled_frame lb sf) (v:=v) 
-      (sigma:=(SIGMA (Labeled_frame lb sf :: s') h)) (s':=s') (s:=(Labeled_frame lb sf :: s')) (h:=h).
-      auto. auto. auto. 
-      case_eq (beq_id x0 x). intro. apply beq_equal with (x:=x0) (x':=x) in H. subst. auto.
-      intro. rewrite -> H in H2. rewrite -> H7 in H2. inversion H2.   
-
-Theorem preservation : forall t t' T sigma sigma', 
-    gamma |- t \in T ->
-    t / st ==> t' / st' ->
-    gamma |- t' \in T.
+  exists s2. exists sigma.
+  apply ST_if_b2 with (sigma:=sigma) (s1:=s1) (s2:=s2) (v1:=v1) (v2:=v2)
+                                (s:=s) (h:=h) (lsf:=lsf) (s':=s') (lb:=lb) (sf:=sf) (id1:=id1) (id2:=id2). 
+  auto. rewrite <- H24 in H4. assumption. auto. auto. auto. intuition.
+  rewrite -> H25 in H30.  rewrite -> H28 in H30. inversion H30.
+  rewrite -> H25 in H30.  rewrite -> H28 in H30. inversion H30.
+  rewrite -> H25 in H30.  rewrite -> H28 in H30. inversion H30.
+  rewrite -> H25 in H30.  rewrite -> H28 in H30. inversion H30.
 
 
-Proof.
+
+destruct H22 with id2 v2.
+  rewrite <- H27.  auto.
+  exists s2. exists sigma.
+  apply ST_if_b2 with (sigma:=sigma) (s1:=s1) (s2:=s2) (v1:=v1) (v2:=v2)
+                                (s:=s) (h:=h) (lsf:=lsf) (s':=s') (lb:=lb) (sf:=sf) (id1:=id1) (id2:=id2). 
+  auto. rewrite <- H24 in H4. assumption. auto. auto. auto. intuition. 
+  rewrite -> H28 in H29. rewrite -> H30 in H29. inversion H29.
+  rewrite -> H28 in H29. rewrite -> H30 in H29. inversion H29.
+  rewrite -> H28 in H29. rewrite -> H30 in H29. inversion H29.
+  rewrite -> H28 in H29. rewrite -> H30 in H29. inversion H29.
+
+destruct H28. destruct H25.  
+
+exists s1. exists sigma.
+  apply ST_if_b1 with (sigma:=sigma) (s1:=s1) (s2:=s2) (v1:=v1) (v2:=v2)
+                                (s:=s) (h:=h) (lsf:=lsf) (s':=s') (lb:=lb) (sf:=sf) (id1:=id1) (id2:=id2). 
+  auto. rewrite <- H24 in H4. assumption. auto. auto. auto. rewrite -> H28. auto.
+
+(* sequence *)
+- right. destruct IHhas_type1. auto. auto. auto.
+   exists e2. exists sigma. 
+   apply ST_seq2 with (sigma:=sigma) (v:=e1) (s:=e2); auto.
+  
+  destruct H2 as [t']. destruct H2 as [sigma'].
+  exists (Sequence t' e2). exists sigma. 
+   apply ST_seq1 with (sigma:=sigma) (s1:=e1) (s2:=e2) (s1':=t'); auto.
+
+(* return e *)
+- right. destruct IHhas_type. auto. auto. auto. 
+  assert (exists lsf s', s = cons lsf s'). 
+  apply stack_not_nil with (sigma:=sigma) (gamma:=Gamma) (CT:=CT) (s:=s) (h:=h).
+  auto. auto. auto.
+  destruct H5 as [lsf]. destruct H5 as [s'].
+  remember (join_label (get_current_label s) (get_current_label s')) as l'.
+  remember (update_current_label s' l' ) as s''.
+  remember (SIGMA s'' h) as sigma'.
+  exists e. exists sigma'.
+  apply ST_return2 with (sigma:=sigma) (sigma':=sigma') (v:=e)
+                                    (s:=s) (s':=s') (s'':=s'') (h:=h) (lsf:=lsf) (l':=l').
+  auto. auto. auto. auto. auto. auto. 
+
+  destruct H4 as [t']. destruct H4 as [sigma'].
+  exists (Return t'). exists sigma'. 
+  apply ST_return1 with (sigma:=sigma) (sigma':=sigma') (e:=e) (e':=t'). auto.
+
+(* ObjId o *)
+- left. apply v_oid. 
+
+(* v_l *)
+- left. apply v_labeled. 
+
+(* v_opl_l *)
+- left. apply v_opa_labeled.
 Qed.
+
+(* reduction preserve well-form of stack and heap *)
+Theorem reduction_preserve_wfe : forall t t' T  sigma sigma' gamma CT s s' h h', 
+    sigma = SIGMA s h ->  wfe_heap CT gamma h -> wfe_stack CT gamma h s -> 
+    has_type CT gamma h t T -> 
+    t / sigma ==> t' / sigma' ->
+    sigma' = SIGMA s' h' ->
+    wfe_heap CT gamma h' /\ wfe_stack CT gamma h' s'.
+Proof with auto. 
+Admitted. 
+
+
+(* reduction preserve typing *)
+
+Theorem preservation : forall t t' T  sigma sigma' gamma CT s s' h h', 
+    sigma = SIGMA s h ->  wfe_heap CT gamma h -> wfe_stack CT gamma h s -> 
+    has_type CT gamma h t T -> 
+    t / sigma ==> t' / sigma' ->
+    sigma' = SIGMA s' h' ->
+    has_type CT gamma h' t' T.
+Proof with auto.
+   intros. 
+   assert (wfe_heap CT gamma h' /\ wfe_stack CT gamma h' s').
+   apply reduction_preserve_wfe with (t:=t) (t':=t') (T:=T)  (sigma:=sigma) (sigma':=sigma') (gamma:=gamma) (CT:=CT) (s:=s) (s':=s') (h:=h) (h':=h').
+   auto. auto. auto. auto. auto. auto.  
+    intros. induction H3.
+- (* Tvar *)
+   inversion H2. inversion H1. rewrite -> H17 in H13. inversion H13. 
+   inversion H18.   destruct H30 with id0 v. inversion H29. inversion H3. 
+      subst. inversion H33.   intuition.                  
+
+rewrite -> H33.
+   apply T_null  with (Gamma:=gamma) (h:=h') (T:= (classTy T0)) (CT:=CT).
+
+   destruct H33.  subst. 
+
+    destruct H34 as [F]. destruct H as [lx]. destruct H as [cls_def0].
+
+assert  (exists cn cls_def, CT cn = Some (cls_def)).
+exists T1. exists cls_def. auto.
+
+assert (exists cn field_defs method_defs, CT cn = Some cls_def0 /\ cls_def0 = (class_def cn field_defs method_defs)).
+
+
+apply heap_consist_ct with (h:=h) (o:=o) (ct:=CT) 
+     (ctx:=(fun x' : id => if beq_id x0 x' then Some (classTy T1) else gamma0 x0))
+     (cls:=cls_def0) (F:=F) (lo:=lx).
+auto.  auto.
+
+destruct H7 as [cls_name]. destruct H7 as [field_defs].  destruct H7 as [method_defs].  destruct H7.  
+
+induction cls_def0.
+ 
+apply T_ObjId with (h:=h') 
+(Gamma:=((fun x' : id => if beq_id x0 x' then Some (classTy T1) else gamma0 x0))) (CT:=CT) (o:=o) 
+                                          (cls_name:=T0) (F:=F) (lo:=lx) (cls_def:=(class_def cls_name field_defs method_defs)).
+auto. inversion H9. rewrite <- H9.  auto. 
+inversion H4. rewrite <- H12. auto. 
+
+- (* FieldAccess *)
+inversion H2. 
+
+
+  | T_FieldAccess : forall Gamma e f cls_def CT clsT cls' h fields_def,
+      has_type CT Gamma h e (classTy clsT) ->       
+      Some cls_def = CT(clsT) ->
+      fields_def = (find_fields cls_def) ->
+      type_of_field fields_def f = Some cls' ->
+      has_type CT Gamma h (FieldAccess e f) (classTy cls')
 
 
 
